src/Term.v
@@ -132,6 +132,13 @@ Definition term_canEqMixin (I B L : eqType) := PcanEqMixin (@pcancel_code_decode
 Canonical term_eqType (I B L : eqType) :=
   Eval hnf in EqType (term I B L) (term_canEqMixin I B L).
 
+Fixpoint get_bs (I B L : eqType) (ts : seq (term I B L)) :=
+  match ts with
+  | nil => nil
+  | Bnode b :: ts' => b :: (get_bs ts')
+  | _ :: ts' => (get_bs ts')
+  end.
+
 Definition term_canChoiceMixin (I B L : choiceType) :=
   PcanChoiceMixin (@pcancel_code_decode I B L).
 
